changed code to use mutable arrays and adapted proofs

libcrux-ml-dsa/src/simd/portable/encoding/commitment.rs
@@ -19,23 +19,27 @@ fn encode_4(coefficients: &[i32]) -> u8 {
 }
 
 #[inline(always)]
-#[hax_lib::requires(fstar!(r"Seq.length ${coefficients} == 4 /\ (forall i. bounded (Seq.index ${coefficients} i) 6)"))]
-#[hax_lib::ensures(|out| fstar!(r"
-let inp = bit_vec_of_int_t_array #I32 #(mk_usize 4) ${coefficients} 6 in
-let out = bit_vec_of_int_t_array #U8 (MkSeq.create3 ${out}) 8 in
-forall (i: nat {i < 8 * 3}). inp i == out i
+#[hax_lib::requires(fstar!(r"Seq.length ${coefficients} == 4 /\ Seq.length ${bytes} == 3 /\ 
+                             (forall i. bounded (Seq.index ${coefficients} i) 6)"))]
+#[hax_lib::ensures(|_| fstar!(r"
+Seq.length ${bytes}_future == Seq.length ${bytes} /\
+(let inp = bit_vec_of_int_t_array #I32 #(mk_usize 4) ${coefficients} 6 in
+ let out = bit_vec_of_int_t_array #U8  #(mk_usize 3) ${bytes}_future 8 in
+ forall (i: nat {i < 8 * 3}). inp i == out i)
 "))]
-fn encode_6(coefficients: &[i32]) -> (u8, u8, u8) {
+fn encode_6(coefficients: &[i32], bytes: &mut [u8]) {
     let coefficient0 = coefficients[0] as u8;
     let coefficient1 = coefficients[1] as u8;
     let coefficient2 = coefficients[2] as u8;
     let coefficient3 = coefficients[3] as u8;
 
-    (
-        (coefficient1 << 6) | coefficient0,
-        (coefficient2 << 4) | coefficient1 >> 2,
-        (coefficient3 << 2) | coefficient2 >> 4,
-    )
+    let byte0 = (coefficient1 << 6) | coefficient0;
+    let byte1 = (coefficient2 << 4) | coefficient1 >> 2;
+    let byte2 = (coefficient3 << 2) | coefficient2 >> 4;
+
+    bytes[0] = byte0;
+    bytes[1] = byte1;
+    bytes[2] = byte2;
 }
 
 #[inline(always)]
@@ -108,10 +112,11 @@ pub fn serialize_6(simd_unit: &Coefficients, serialized: &mut [u8]) {
             )
         });
 
-        let (r0, r1, r2) = encode_6(coefficients);
-        serialized[3 * i] = r0;
-        serialized[3 * i + 1] = r1;
-        serialized[3 * i + 2] = r2;
+        // TODO: use ghost state here to avoid copying
+        // See: https://github.com/cryspen/libcrux/issues/783
+        let mut _old_serialized: [u8; 6] = core::array::from_fn(|i| serialized[i]);
+
+        encode_6(coefficients, &mut serialized[3 * i..3 * i + 3]);
 
         hax_lib::fstar!(
             r"
@@ -127,7 +132,14 @@ pub fn serialize_6(simd_unit: &Coefficients, serialized: &mut [u8]) {
                 == {} get_bit (Seq.index $coefficients (n / 6)) (sz (n % 6));
                 == {} bit_vec_of_int_t_array #I32 #(mk_usize 4) $coefficients 6 n;
                 == {} out (v i * 24 + n);
-                })
+                });
+           (* Find a better style for these sequence updates so that such silly assertions become unnecessary *)
+           assert (forall (n:nat{n >= 24 * v i /\ n < 24 * v i + 24}). inp (24 * v i + (n - 24 * v i)) == out (24 * v i + (n - 24 * v i)));
+           assert (forall (n:nat{n >= 24 * v i /\ n < 24 * v i + 24}). inp n == out n);
+           assert (forall (n:nat{n < v i * 24}). n / 8 < 3 * v i);
+           assert (forall (j:nat{j < 3 * v i}). Seq.index ${serialized} j == Seq.index (Seq.slice ${serialized} 0 (3 * v i)) j);
+           assert (forall (j:nat{j < 3 * v i}). Seq.index ${_old_serialized} j == Seq.index (Seq.slice ${_old_serialized} 0 (3 * v i)) j);
+           assert (forall (n:nat{n < 24 * (v i + 1)}). inp n == out n))
         "
         );
     }
