libcrux-ml-dsa/proofs/fstar/extraction/Libcrux_ml_dsa.Simd.Portable.Encoding.Commitment.fsti
@@ -13,15 +13,18 @@ val encode_4_ (coefficients: t_Slice i32)
           let out = bit_vec_of_int_t_array #U8 (MkSeq.create1 out) 8 in
           forall (i: nat{i < 8}). inp i == out i)
 
-val encode_6_ (coefficients: t_Slice i32)
-    : Prims.Pure (u8 & u8 & u8)
-      (requires Seq.length coefficients == 4 /\ (forall i. bounded (Seq.index coefficients i) 6))
+val encode_6_ (coefficients: t_Slice i32) (bytes: t_Slice u8)
+    : Prims.Pure (t_Slice u8)
+      (requires
+        Seq.length coefficients == 4 /\ Seq.length bytes == 3 /\
+        (forall i. bounded (Seq.index coefficients i) 6))
       (ensures
-        fun out ->
-          let out:(u8 & u8 & u8) = out in
-          let inp = bit_vec_of_int_t_array #I32 #(mk_usize 4) coefficients 6 in
-          let out = bit_vec_of_int_t_array #U8 (MkSeq.create3 out) 8 in
-          forall (i: nat{i < 8 * 3}). inp i == out i)
+        fun bytes_future ->
+          let bytes_future:t_Slice u8 = bytes_future in
+          Seq.length bytes_future == Seq.length bytes /\
+          (let inp = bit_vec_of_int_t_array #I32 #(mk_usize 4) coefficients 6 in
+            let out = bit_vec_of_int_t_array #U8 #(mk_usize 3) bytes_future 8 in
+            forall (i: nat{i < 8 * 3}). inp i == out i))
 
 val serialize_4_
       (simd_unit: Libcrux_ml_dsa.Simd.Portable.Vector_type.t_Coefficients)
